@prefix owl: <http://www.w3.org/2002/07/owl#> .
@prefix geo: <http://www.w3.org/2003/01/geo/wgs84_pos#> .
@prefix rdfs: <http://www.w3.org/2000/01/rdf-schema#> .
@prefix dc: <http://purl.org/dc/elements/1.1/> . 
@prefix dct: <http://purl.org/dc/terms/> .
@prefix schema: <https://schema.org/> .
@prefix foaf: <http://xmlns.com/foaf/0.1/> .
@prefix xsd: <http://www.w3.org/2001/XMLSchema#> .
@prefix vann: <http://purl.org/vocab/vann/> .
@prefix sosa: <http://www.w3.org/ns/sosa/> .
@prefix prov: <http://www.w3.org/ns/prov#> . 
@prefix qudt: <http://qudt.org/schema/qudt/>.

@prefix emobon-core: <https://data.emobon.embrc.eu/ns/core#> .
@prefix emobon-sampling: <https://data.emobon.embrc.eu/ns/sampling#> .
@prefix emobon-sequence: <https://data.emobon.embrc.eu/ns/sequence#> .

<https://data.emobon.embrc.eu/ns/sampling>
  a owl:Ontology ;
  owl:versionIRI <https://data.emobon.embrc.eu/ns/sampling.ttl> ;
  foaf:homepage  <https://marineregions.org/ontology/documentation.html> ;
  rdfs:label     "The Sampling EMO-BON Ontology"@en ;
  rdfs:comment   "The Sampling EMO-BON ontology provides definitions for the sampling classes and properties used in EMO-BON data."@en ;
  dc:publisher   <https://www.vliz.be/> ;
  dct:issued      "2023-03-17"^^xsd:date ;
  dct:modified    "2023-07-26"^^xsd:date ;
  dc:license     <https://creativecommons.org/licenses/by/4.0/> ;
  dc:contributor 
    <https://orcid.org/0000-0001-7251-9504>,
    <https://orcid.org/0000-0002-5911-1536>,
    <https://orcid.org/0000-0003-0663-5907>;
  dc:creator <https://www.embrc.eu> ;
  vann:preferredNamespacePrefix "emobon-sampling" ;
  vann:preferredNamespaceUri    "https://data.emobon.embrc.eu/ns/sampling#" .

<https://orcid.org/0000-0001-7251-9504>
        foaf:name         "Henriette Harmse" ;
        schema:identifier   <https://orcid.org/0000-0001-7251-9504> ;
        schema:email        <mailto:henriette007@ebi.ac.uk> ;
        schema:affiliation  <https://www.embrc.eu> ;
.

<https://orcid.org/0000-0002-5911-1536>
  a schema:Person ; 
  foaf:name         "Katrina Exter" ;
  schema:identifier   <https://orcid.org/0000-0002-5911-1536> ;
  schema:email        <mailto:katrina.exter@vliz.be> ;
  schema:affiliation  <https://www.vliz.be> ;
.

<https://orcid.org/0000-0003-0663-5907>
  a schema:Person ;
  foaf:name         "Laurian Van Maldeghem" ;
  schema:identifier   <https://orcid.org/0000-0003-0663-5907> ;
  schema:email        <mailto:laurian.van.maldeghem@vliz.be> ;
  schema:affiliation  <https://www.vliz.be> ;
.

<https://www.vliz.be/>
  a schema:Organization ;
  schema:name   "Vlaams Instituut voor de Zee"@nl ;
  schema:name   "Flanders Marine Institute"@en ;
  schema:url    <https://www.vliz.be/> ;
.

<https://www.embrc.eu>
  a schema:Organization ;
  schema:name   "European Marine Biological Resource Centre"@en ;
  schema:url    <https://www.embrc.eu> ;
.


#### CLASSES Sample ####
<https://data.emobon.embrc.eu/ns/sampling#siteInfo>
    a owl:Class ; 
    rdfs:isDefinedBy <https://data.emobon.embrc.eu/ns/sampling> ;
    rdfs:comment "Extra information on the sampling site, in particular concerning other data collections from the same area, environmental activities or events, etc." ; 
    rdfs:label "Sampling site information" ; 
    rdfs:subClassOf rdfs:comment ;
.


#### PROPERTIES Sample ####
<https://data.emobon.embrc.eu/ns/sampling#origEmobonId
    a                     owl:DatatypeProperty ;
    rdfs:isDefinedBy      <https://data.emobon.embrc.eu/ns/sampling> ;
    rdfs:comment          "The original EMOBON assigned identifier as used for the sample material."@en ;
    rdfs:label            "original EMOBON assigned identifier"@en ;
    rdfs:domain           sosa:Sampling ;
    rdfs:range            xsd:string ;
.

<https://data.emobon.embrc.eu/ns/sampling#linkedToObservatory> 
    a                     owl:ObjectProperty ;
    rdfs:isDefinedBy      <https://data.emobon.embrc.eu/ns/sampling> ;
    rdfs:comment          "The observatory that is linked to the sampling event."@en ;
    rdfs:label            "is linked to observatory"@en ;
    rdfs:domain           sosa:Sampling ;
    rdfs:range            emobon-core:Observatory ;
.

<https://data.emobon.embrc.eu/ns/sampling#enaProjAccNum>
    a                   owl:DatatypeProperty ;
    rdfs:isDefinedBy    <https://data.emobon.embrc.eu/ns/sampling> ;
    rdfs:comment        "ENA project accession number associated to this observatory."@en ;
    rdfs:label          "has ENA project accession number"@en ;
    rdfs:domain         schema:Project ;
    rdfs:range          xsd:string ;
.

<https://data.emobon.embrc.eu/ns/sampling#enaStudyAccNum>
    a                   owl:DatatypeProperty ;
    rdfs:isDefinedBy    <https://data.emobon.embrc.eu/ns/sampling> ;
    rdfs:comment        "ENA study accession number associated to the observatory."@en ;
    rdfs:label          "has ENA study accession number"@en ;
    rdfs:domain         emobon-core:Observatory ;
    rdfs:range          xsd:string ;
.

<https://data.emobon.embrc.eu/ns/sampling#enaSampleAccNum>
    a                   owl:DatatypeProperty ;
    rdfs:isDefinedBy    <https://data.emobon.embrc.eu/ns/sampling> ;
    rdfs:comment        "ENA sample accession number associated with the sample."@en ;
    rdfs:label          "has ENA sample accession number"@en ;
    rdfs:domain         sosa:Sample ;
    rdfs:range          xsd:string ;
.

<https://data.emobon.embrc.eu/ns/sampling#hasMixsPackage>
    a                   owl:DatatypeProperty ;
    rdfs:isDefinedBy    <https://data.emobon.embrc.eu/ns/sampling> ;
    rdfs:comment        "The MIxS extension for reporting of measurements and observations obtained from one or more of the environments where a sample was obtained"@en ;
    rdfs:label          "has Mixs Package"@en ;
    rdfs:domain         emobon-core:Observatory ;
    rdfs:range          xsd:string ;
.

<https://data.emobon.embrc.eu/ns/sampling#originCountry>
    a                   owl:DatatypeProperty ;
    rdfs:isDefinedBy    <https://data.emobon.embrc.eu/ns/sampling> ;
    rdfs:comment        "The geographical origin of the sample as defined by the country name."@en ;
    rdfs:label          "Country of origin of the sample"@en ;
    rdfs:domain         [
                            a owl:Class ; 
                            owl:unionOf (
                                sosa:Sampling
                                emobon-core:Observatory
                            ) ; 
                        ] ;
    rdfs:range          xsd:string ;
.

<https://data.emobon.embrc.eu/ns/sampling#soilType>
    a                   owl:DatatypeProperty ;
    rdfs:isDefinedBy    <https://data.emobon.embrc.eu/ns/sampling> ;
    rdfs:comment        "Information about the sediment type of the sample based on major constituents"@en ;
    rdfs:label          "Sediment type of a soil sample"@en ;
    rdfs:domain         emobon-core:Observatory ;
    rdfs:range          xsd:string ;
.

<https://data.emobon.embrc.eu/ns/sampling#environmentMaterial>
    a                   owl:DatatypeProperty ;
    rdfs:isDefinedBy    <https://data.emobon.embrc.eu/ns/sampling> ;
    rdfs:comment        "The physical material being collected"@en ;
    rdfs:label          "Environment material"@en ;
    rdfs:domain         sosa:Sampling , sosa:Sample ;
    rdfs:range          xsd:string ;
.

<https://data.emobon.embrc.eu/ns/sampling#investigationType>
    a                   owl:DatatypeProperty ;
    rdfs:isDefinedBy    <https://data.emobon.embrc.eu/ns/sampling> ;
    rdfs:comment        "Describes what is intended to be done with the Environment material, i.e. the type of organisms to be investigated in that material"@en ;
    rdfs:label          "Investigation type"@en ;
    rdfs:domain         sosa:Sampling , sosa:Sample ;
    rdfs:range          xsd:string ;
.

<https://data.emobon.embrc.eu/ns/sampling#minSamplingDepth>
    a                   owl:DatatypeProperty ;
    rdfs:isDefinedBy    <https://data.emobon.embrc.eu/ns/sampling> ;
    rdfs:comment        "Measument of the sampling depth of the water column in meters"@en ;
    rdfs:label          "Sampling depth of water column"@en ;
    rdfs:domain         sosa:Sampling;
    rdfs:range          qudt:QuantityValue ;
.

<https://data.emobon.embrc.eu/ns/sampling#maxSamplingDepth>
    a                   owl:DatatypeProperty ;
    rdfs:isDefinedBy    <https://data.emobon.embrc.eu/ns/sampling> ;
    rdfs:comment        "Measument of the maximum sampling depth of the water column in meters"@en ;
    rdfs:label          "Max sampling depth of water column"@en ;
    rdfs:domain         sosa:Sampling;
    rdfs:range          qudt:QuantityValue ;
.


<https://data.emobon.embrc.eu/ns/sampling#minSampleDepth>
    a                   owl:DatatypeProperty ; 
    rdfs:isDefinedBy    <https://data.emobon.embrc.eu/ns/sampling> ;
    rdfs:comment        "Measument of the minimum sample depth of the water column in meters"@en ;
    rdfs:label          "Min sampling depth of water column"@en ;
    rdfs:domain         sosa:Sample;
    rdfs:range          qudt:QuantityValue ;
.

<https://data.emobon.embrc.eu/ns/sampling#maxSampleDepth>
    a                   owl:DatatypeProperty ; 
    rdfs:isDefinedBy    <https://data.emobon.embrc.eu/ns/sampling> ;
    rdfs:comment        "Measument of the maximum sample depth of the water column in meters"@en ;
    rdfs:label          "Max sampling depth of water column"@en ;
    rdfs:domain         sosa:Sample;
    rdfs:range          qudt:QuantityValue ;
.

<https://data.emobon.embrc.eu/ns/sampling#tidalStage>
    a                   owl:DatatypeProperty ;
    rdfs:isDefinedBy    <https://data.emobon.embrc.eu/ns/sampling> ;
    rdfs:comment        "Tidal stage at the moment of the sampling event, expected values are: low_tide, ebb_tide, flood_tide, high_tide"@en ;
    rdfs:label          "Tidal stage"@en ;
    rdfs:domain         sosa:Sampling;
    rdfs:range          xsd:string ;
.

<https://data.emobon.embrc.eu/ns/sampling#storageTemp>
    a                   owl:DatatypeProperty ;
    rdfs:isDefinedBy    <https://data.emobon.embrc.eu/ns/sampling> ;
    rdfs:comment        "Temperature at which the sample was stored during a storage activity."@en ;
    rdfs:label          "Storage temperature"@en ;
    rdfs:domain         prov:Activity ;
    rdfs:range          qudt:QuantityValue ;
.

<https://data.emobon.embrc.eu/ns/sampling#storageLoc>
    a                   owl:DatatypeProperty ;
    rdfs:isDefinedBy    <https://data.emobon.embrc.eu/ns/sampling> ;
    rdfs:comment        "Location at which the sample was stored during a storage activity."@en ;
    rdfs:label          "Storage location"@en ;
    rdfs:domain         prov:Activity ;
    rdfs:range          xsd:string ;
.

<https://data.emobon.embrc.eu/ns/sampling#longStorage>
    a                   owl:DatatypeProperty ;
    rdfs:isDefinedBy    <https://data.emobon.embrc.eu/ns/sampling> ;
    rdfs:comment        "Indicates if the sample is stored long term."@en ;
    rdfs:label          "Long storage"@en ;
    rdfs:domain         sosa:Sample ;
    rdfs:range          xsd:boolean ;
.

<https://data.emobon.embrc.eu/ns/sampling#membrCut>
    a                   owl:DatatypeProperty ;
    rdfs:isDefinedBy    <https://data.emobon.embrc.eu/ns/sampling> ;
    rdfs:comment        "Indicates if the membrane was cut in half after filtration"@en ;
    rdfs:label          "Membrane cut"@en ;
    rdfs:domain         sosa:Sample ;
    rdfs:range          xsd:boolean ;
.

## note on range: most values will be xsd:float, but xsd:string also in data (see term definition) 
<https://data.emobon.embrc.eu/ns/sampling#filtrationTime>
    a                   owl:DatatypeProperty ;
    rdfs:isDefinedBy    <https://data.emobon.embrc.eu/ns/sampling> ;
    rdfs:comment        "Indicates how long from sampling until start of filtration, 'fi' indicates filtration was done in the field."@en ;
    rdfs:label          "Filtration time"@en ;
    rdfs:domain         sosa:Sample ;
    rdfs:range          qudt:QuantityValue ;
.

<https://data.emobon.embrc.eu/ns/sampling#hasSampleSize>
    a                   owl:DatatypeProperty ;
    rdfs:isDefinedBy    <https://data.emobon.embrc.eu/ns/sampling> ;
    rdfs:comment        "The size of the collected sample"@en ;
    rdfs:label          "has ENA sample accession number"@en ;
    rdfs:domain         sosa:Sample ;
    rdfs:range          qudt:QuantityValue ;
.

#note: if values could be converted to T ~ true|1 and F ~ false|0 then datatype can be xsd:boolean
<https://data.emobon.embrc.eu/ns/sampling#failure>
    a                   owl:DatatypeProperty ;
    rdfs:isDefinedBy    <https://data.emobon.embrc.eu/ns/sampling> ;
    rdfs:comment        "Indication of failure in data generation, which may have occured at any stage of the workflow; takes True (T) or False (F) values."@en ;
    rdfs:label          "sample failure"@en ;
    rdfs:domain         sosa:Sample ;
    rdfs:range          xsd:string ; 
.

<https://data.emobon.embrc.eu/ns/sampling#failureComment>
    a                   owl:DatatypeProperty ;
    rdfs:isDefinedBy    <https://data.emobon.embrc.eu/ns/sampling> ;
    rdfs:comment        "Desciption of failure cause"@en ;
    rdfs:label          "sample failure comment"@en ;
    rdfs:domain         sosa:Sample ;
    rdfs:range          xsd:string ; 
.

<https://data.emobon.embrc.eu/ns/sampling#sampleReplicate>
    a                   owl:DatatypeProperty ;
    rdfs:isDefinedBy    <https://data.emobon.embrc.eu/ns/sampling> ;
    rdfs:comment        "Replicate number of the sample or Blank"@en ;
    rdfs:label          "sample replicate"@en ;
    rdfs:domain         sosa:Sample ;
    rdfs:range          xsd:string ; 
.

<https://data.emobon.embrc.eu/ns/sampling#filterSizeRange>
    a                   owl:DatatypeProperty ;
    rdfs:isDefinedBy    <https://data.emobon.embrc.eu/ns/sampling> ;
    rdfs:comment        "The Range of sieve pore size used to pre-filter/pre-sort and retain the macrobenthos sample."@en ;
    rdfs:label          "filter size range"@en ;
    rdfs:domain         sosa:Sample ;
    rdfs:range          xsd:string ; 
.

<https://data.emobon.embrc.eu/ns/sampling#lowerFilterSize>
    a                   owl:DatatypeProperty ;
    rdfs:isDefinedBy    <https://data.emobon.embrc.eu/ns/sampling> ;
    rdfs:comment        "The sieve pore size used to pre-filter/pre-sort the macrobenthos sample. Materials larger than the size threshold are excluded from the sample."@en ;
    rdfs:label          "lower filter size"@en ;
    rdfs:domain         sosa:Sample ;
    rdfs:range          qudt:QuantityValue ; 
.

<https://data.emobon.embrc.eu/ns/sampling#upperFilterSize>
    a                   owl:DatatypeProperty ;
    rdfs:isDefinedBy    <https://data.emobon.embrc.eu/ns/sampling> ;
    rdfs:comment        "The sieve pore size used to retain the macrobenthos sample. Materials smaller than the size threshold are excluded from the sample"@en ;
    rdfs:label          "upper filter size"@en ;
    rdfs:domain         sosa:Sample ;
    rdfs:range          qudt:QuantityValue ; 
.